model_properties/inf_buffer_compatible.dfy
@@ -3,30 +3,39 @@ predicate sorted(s: seq<real>)
     forall j, k :: 0 <= j <= k < |s| ==> s[j] <= s[k] 
 }
 
+// If all neighbors are in sorted order, 'sorted' is true
+lemma SortedNeighbor(s: seq<real>)
+requires forall i :: 0 <= i < i + 1 < |s| ==> s[i] <= s[i+1]
+ensures sorted(s)
+{
+    forall j, k | 0 <= j <= k < |s| {
+        SortedNeighborHelper(s, j, k);
+    }
+}
+
+lemma SortedNeighborHelper(s: seq<real>, j: nat, k: nat)
+requires forall i :: 0 <= i < i + 1 < |s| ==> s[i] <= s[i+1]
+requires 0 <= j <= k < |s|
+ensures s[j] <= s[k] {
+    var i := j;
+    while i < k 
+    invariant 0 <= j <= i <= k <= |s|
+    invariant s[j] <= s[i]
+    {
+        i := i + 1;
+    }
+}
+
 predicate bounded_topps(opps: seq<real>, C: real, ku: real, kl: real)
 {
     sorted(opps) && 
     forall t :: 0 <= t < |opps| ==> t as real * C - kl <= opps[t] <= t as real * C + ku
 }
 
-/*lemma LemmaBoundedToppsConcat(opps1: seq<real>, opps2: seq<real>, C: real, ku: real, kl: real)
-decreases opps1
-requires bounded_topps(opps1, C, ku, kl)
-requires bounded_topps(opps2, C, ku, kl)
-ensures bounded_topps(opps1 + seq_add(opps2, C * |opps1| as real), C, ku, kl)
-{
-    if |opps1| == 0 {
-        assert seq_add(opps2, 0.0) == opps2;
-        assert opps1 + seq_add(opps2, C * |opps1| as real) == opps2;
-    } else {
-
-        var x := C * |opps1| as real;
-        assert seq_add([opps1[|opps1|-1] - x] + opps2, x) == [opps1[|opps1|-1]] + seq_add(opps2, x);
-        assert opps1 + seq_add(opps2, C * |opps1| as real) ==
-            opps1[..|opps1|-1] + seq_add([opps1[|opps1|-1] - x] + opps2, x);
-        LemmaBoundedToppsConcat(opps1[..|opps1|-1], [opps1[|opps1|-1] - x] + opps2, C, ku, kl);
-    }
-}*/
+function run_inf_link(inp: seq<real>, opps: seq<real>) : (out: seq<real>)
+requires sorted(inp)
+requires sorted(opps)
+{}
 
 // Definition of a link with an infinitely large buffer
 /*method run_inf_link(inp: array<int>, opps: array<int>) returns (out: array<int>) 
@@ -70,24 +79,11 @@ ensures forall i :: 0 <= i < |inp| ==> inp[i] + val == out[i]
         [inp[0] + val] + seq_add(inp[1..], val)
 }
 
-// A constant bit rate link
-/*method link_cbr(C: real, t: nat) returns (opps: seq<real>)
-    requires C > 0.0
-    ensures sorted(opps)
-    ensures forall ku, kl :: && 0.0 <= ku && 0.0 <= kl ==> bounded_topps(opps, C, ku, kl)
-{
-    if t == 0 {
-        return [];
-    }
-    var tail := link_cbr(C, t-1);
-    return [0.0] + seq_add(tail, C);
-}*/
-
-method link_cbr(inp: seq<real>, C: real) returns (out: seq<real>)
+method link_cbr(inp: seq<real>, C: real) returns (opps: seq<real>)
     requires sorted(inp)
-    requires |inp| == 0 || inp[0] >= 0.0
+    requires |inp| > 0 ==> inp[0] >= 0.0
     requires C > 0.0
-    ensures bounded_topps(out, C, 0.0, 0.0)
+    ensures bounded_topps(opps, C, 0.0, 0.0)
 {
     if |inp| == 0 {
         return [];
@@ -126,4 +122,38 @@ method link_cbr(inp: seq<real>, C: real) returns (out: seq<real>)
         res[t] := t as real * C;
     }
     return res[..];
+}
+
+// Implements a link of the given rate that sends a burst every 
+// 'agg' timesteps
+method link_aggr(tot_timesteps: nat, C: real, agg: nat) returns (opps: seq<real>)
+requires agg > 0
+requires C > 0.0
+ensures bounded_topps(opps, C, 0.0, C  * agg as real)
+{
+    var res := new real[tot_timesteps];
+    var t := 0;
+    while t < tot_timesteps 
+    invariant 0 <= t <= tot_timesteps
+    invariant forall i :: 0 <= i < t ==> res[i] == C * ((i / agg) * agg) as real
+    {
+        res[t] := C * ((t / agg) * agg) as real;
+        t := t + 1;
+    }
+
+    opps := res[..];
+
+    // Prove that it is sorted
+    forall t | 0 <= t < t + 1 < |opps| 
+    ensures opps[t] <= opps[t+1];
+    {
+        assert t <= t + 1;
+        assert t / agg <= (t + 1) / agg;
+        assert agg > 0;
+        assert (t / agg) * agg <= ((t+1) / agg) * agg;
+    }
+    SortedNeighbor(opps);
+    assert sorted(opps);
+
+    return opps;
 }
